src/lib/kernel/gemm/Kuiper.Kernel.GEMM.TensorCore2D.KernelDesc.fst
@@ -32,24 +32,24 @@ open Pulse.Lib.Trade
 module SZ = Kuiper.SizeT
 
 let bid_of_ij
-  (rows cols : nat)
-  (bm : pos{bm /?+ rows})
-  (bn : pos{bn /?+ cols})
-  (i : natlt rows)
-  (j : natlt cols)
-  : natlt (rows/bm * (cols/bn))
-  = (i / bm) * (cols/bn) + (j / bn)
+  (m n : nat)
+  (bm : pos{bm /?+ m})
+  (bn : pos{bn /?+ n})
+  (i : natlt m)
+  (j : natlt n)
+  : natlt (m/bm * (n/bn))
+  = (i / bm) * (n/bn) + (j / bn)
 
 let wid_of_ij
-  (rows cols : nat)
-  (bm : pos{bm /?+ rows})
-  (bn : pos{bn /?+ cols})
+  (m n : nat)
+  (bm : pos{bm /?+ m})
+  (bn : pos{bn /?+ n})
   (tm : pos{tm /?+ bm})
   (tn : pos{tn /?+ bn})
   (wm : pos{wm * tm /?+ bm})
   (wn : pos{wn * tn /?+ bn})
-  (i : natlt rows)
-  (j : natlt cols)
+  (i : natlt m)
+  (j : natlt n)
   : natlt (bm/(wm*tm) * (bn/(wn*tn)))
   =
     let i0 : natlt (bm/(wm*tm)) = (i % bm) / (wm*tm) in
@@ -67,32 +67,32 @@ let silly_div_helper (p : pos)
   = ()
 
 let lem_i
-  (rows shared cols : nat)
+  (m n k : nat)
   (bm bn bk
    tm tn tk
    wm wn : pos { constraints bm bn bk tm tn tk wm wn })
-  (#_ : squash (bm /?+ rows))
-  (#_ : squash (bn /?+ cols))
+  (#_ : squash (bm /?+ m))
+  (#_ : squash (bn /?+ n))
   (nthr : pos{nthr == bm/(wm*tm) * (bn/(wn*tn)) * warp_size})
-  (i : natlt rows)
-  (j : natlt cols)
-  : Lemma (ensures warp_tile_i #rows #cols bm bn bk tm tn tk wm wn
+  (i : natlt m)
+  (j : natlt n)
+  : Lemma (ensures warp_tile_i #m #n bm bn bk tm tn tk wm wn
                        nthr
-                       (bid_of_ij rows cols bm bn i j)
-                       (wid_of_ij rows cols bm bn tm tn wm wn i j)
+                       (bid_of_ij m n bm bn i j)
+                       (wid_of_ij m n bm bn tm tn wm wn i j)
                      * (wm*tm) + ((i % bm) % (wm*tm)) == i)
-  = let bid = bid_of_ij rows cols bm bn i j in
-    let wid = wid_of_ij rows cols bm bn tm tn wm wn i j in
-    assert (j/bn < cols/bn);
-    silly_modulo_helper (cols/bn) (i/bm) (j/bn);
-    assert (bid / (cols/bn) == i / bm);
+  = let bid = bid_of_ij m n bm bn i j in
+    let wid = wid_of_ij m n bm bn tm tn wm wn i j in
+    assert (j/bn < n/bn);
+    silly_modulo_helper (n/bn) (i/bm) (j/bn);
+    assert (bid / (n/bn) == i / bm);
     silly_div_helper (bn/(wn*tn)) ((i%bm)/(wm*tm)) ((j%bn)/(wn*tn));
     assert (wid / (bn/(wn*tn)) == (i % bm) / (wm*tm));
     calc (==) {
-      warp_tile_i #rows #cols bm bn bk tm tn tk wm wn nthr bid wid * (wm*tm)
+      warp_tile_i #m #n bm bn bk tm tn tk wm wn nthr bid wid * (wm*tm)
         + ((i % bm) % (wm*tm));
       == {}
-      ((bid / (cols/bn)) * (bm / (wm*tm)) + wid / (bn/(wn*tn))) * (wm*tm)
+      ((bid / (n/bn)) * (bm / (wm*tm)) + wid / (bn/(wn*tn))) * (wm*tm)
         + ((i % bm) % (wm*tm));
       == {}
       ((i/bm) * (bm / (wm*tm)) + wid / (bn/(wn*tn))) * (wm*tm)
@@ -111,32 +111,32 @@ let lem_i
     ()
 
 let lem_j
-  (rows shared cols : nat)
+  (m n k : nat)
   (bm bn bk
    tm tn tk
    wm wn : pos { constraints bm bn bk tm tn tk wm wn })
-  (#_ : squash (bm /?+ rows))
-  (#_ : squash (bn /?+ cols))
+  (#_ : squash (bm /?+ m))
+  (#_ : squash (bn /?+ n))
   (nthr : pos{nthr == bm/(wm*tm) * (bn/(wn*tn)) * warp_size})
-  (i : natlt rows)
-  (j : natlt cols)
-  : Lemma (ensures warp_tile_j #rows #cols bm bn bk tm tn tk wm wn
+  (i : natlt m)
+  (j : natlt n)
+  : Lemma (ensures warp_tile_j #m #n bm bn bk tm tn tk wm wn
                        nthr
-                       (bid_of_ij rows cols bm bn i j)
-                       (wid_of_ij rows cols bm bn tm tn wm wn i j)
+                       (bid_of_ij m n bm bn i j)
+                       (wid_of_ij m n bm bn tm tn wm wn i j)
                      * (wn*tn) + ((j % bn) % (wn*tn)) == j)
-  = let bid = bid_of_ij rows cols bm bn i j in
-    let wid = wid_of_ij rows cols bm bn tm tn wm wn i j in
-    assert (j/bn < cols/bn);
-    silly_modulo_helper (cols/bn) (i/bm) (j/bn);
-    assert (bid % (cols/bn) == j / bn);
+  = let bid = bid_of_ij m n bm bn i j in
+    let wid = wid_of_ij m n bm bn tm tn wm wn i j in
+    assert (j/bn < n/bn);
+    silly_modulo_helper (n/bn) (i/bm) (j/bn);
+    assert (bid % (n/bn) == j / bn);
     silly_div_helper (bn/(wn*tn)) ((i%bm)/(wm*tm)) ((j%bn)/(wn*tn));
     assert (wid % (bn/(wn*tn)) == (j % bn) / (wn*tn));
     calc (==) {
-      warp_tile_j #rows #cols bm bn bk tm tn tk wm wn nthr bid wid * (wn*tn)
+      warp_tile_j #m #n bm bn bk tm tn tk wm wn nthr bid wid * (wn*tn)
         + ((j % bn) % (wn*tn));
       == {}
-      ((bid % (cols/bn)) * (bn/(wn*tn)) + wid % (bn/(wn*tn))) * (wn*tn)
+      ((bid % (n/bn)) * (bn/(wn*tn)) + wid % (bn/(wn*tn))) * (wn*tn)
         + ((j % bn) % (wn*tn));
       == {}
       ((j/bn) * (bn/(wn*tn)) + wid % (bn/(wn*tn))) * (wn*tn)
@@ -193,11 +193,11 @@ fn gpu_slice_gather_underspec
 ghost
 fn gpu_matrix_share_threads
   (#et : Type)
-  (#rows #cols : nat)
-  (#l : mlayout rows cols)
+  (#m #n : nat)
+  (#l : mlayout m n)
   (gm : gpu_matrix et l)
   (#f : perm)
-  (#em : ematrix et rows cols)
+  (#em : ematrix et m n)
   (nblk nthr : pos)
 requires
   gm |-> Frac f em
@@ -213,32 +213,32 @@ fn setup
   (#et_ab #et_c : Type0)
   {| scalar et_ab, scalar et_c |}
   {| real_like et_ab, real_like et_c |}
-  (#rows #shared #cols : szp)
-  (#lA : mlayout rows shared)
-  (#lB : mlayout shared cols)
-  (#lC : mlayout rows cols)
+  (#m #n #k : szp)
+  (#lA : mlayout m k)
+  (#lB : mlayout k n)
+  (#lC : mlayout m n)
   {| clayout lA, clayout lB, clayout lC |}
   (gA : gpu_matrix et_ab lA)
-  (eA : ematrix et_ab rows shared)
+  (eA : ematrix et_ab m k)
   (gB : gpu_matrix et_ab lB)
-  (eB : ematrix et_ab shared cols)
+  (eB : ematrix et_ab k n)
   (gC : gpu_matrix et_c lC)
-  (eC : ematrix et_c rows cols)
+  (eC : ematrix et_c m n)
   (bm bn bk
    tm tn tk
    wm wn : szp { constraints bm bn bk tm tn tk wm wn })
-  (#_ : squash (bm /? rows))
-  (#_ : squash (bk /?+ shared))
-  (#_ : squash (bn /? cols))
+  (#_ : squash (bm /? m))
+  (#_ : squash (bk /?+ k))
+  (#_ : squash (bn /? n))
   (#_ : squash (SZ.fits (bm * bk) /\ SZ.fits (bk * bn)))
   (#_ : squash (aligned 16 (core gA)))
   (#_ : squash (aligned 16 (core gB)))
-  (nblk : szp{SZ.v nblk == rows/bm * (cols/bn)})
+  (nblk : szp{SZ.v nblk == m/bm * (n/bn)})
   (nthr : szp{SZ.v nthr == bm/(wm*tm) * (bn/(wn*tn)) * warp_size})
   (fA fB : perm)
-  (rA : ematrix real rows shared)
-  (rB : ematrix real shared cols)
-  (rC : ematrix real rows cols)
+  (rA : ematrix real m k)
+  (rB : ematrix real k n)
+  (rC : ematrix real m n)
   ()
   norewrite
   requires
@@ -256,19 +256,19 @@ fn setup
   gpu_matrix_share_threads gB nblk nthr;
 
   gpu_matrix_tile gC bm bn;
-  forevery_unfactor' nblk (rows/bm) (cols/bn) _;
+  forevery_unfactor' nblk (m/bm) (n/bn) _;
 
   ghost
   fn create_warp_tiles_shared
     (#et : Type0) {| scalar et |}
-    (#rows #cols : nat)
-    (#l : mlayout rows cols)
+    (#m #n : nat)
+    (#l : mlayout m n)
     ([@@@mkey] gm : gpu_matrix et l)
     (#f : perm)
-    (#em : ematrix et rows cols)
-    (trows : nat{trows > 0 /\ trows /? rows})
-    (tcols : nat{tcols > 0 /\ tcols /? cols})
-    (nthr : nat{nthr == rows/trows * (cols/tcols) * warp_size})
+    (#em : ematrix et m n)
+    (trows : nat{trows > 0 /\ trows /? m})
+    (tcols : nat{tcols > 0 /\ tcols /? n})
+    (nthr : nat{nthr == m/trows * (n/tcols) * warp_size})
   requires
     gm |-> Frac f em
   ensures
@@ -276,35 +276,35 @@ fn setup
       warp_tile gm trows tcols (trc/warp_size)
         |-> Frac (f /. warp_size)
       (ematrix_subtile em trows tcols
-        (warp_tile_idx_rows rows cols trows tcols (trc/warp_size))
-        (warp_tile_idx_cols rows cols trows tcols (trc/warp_size)))
+        (warp_tile_idx_rows m n trows tcols (trc/warp_size))
+        (warp_tile_idx_cols m n trows tcols (trc/warp_size)))
   {
     gpu_matrix_tile gm trows tcols;
-    forevery_unfactor' (rows/trows * (cols/tcols)) (rows/trows) (cols/tcols) _;
+    forevery_unfactor' (m/trows * (n/tcols)) (m/trows) (n/tcols) _;
 
     forevery_map
-      (fun (trc : natlt (rows/trows * (cols/tcols))) ->
-        gpu_matrix_subtile gm trows tcols (trc/(cols/tcols)) (trc%(cols/tcols))
-          |-> Frac f (ematrix_subtile em trows tcols (trc/(cols/tcols)) (trc%(cols/tcols))))
+      (fun (trc : natlt (m/trows * (n/tcols))) ->
+        gpu_matrix_subtile gm trows tcols (trc/(n/tcols)) (trc%(n/tcols))
+          |-> Frac f (ematrix_subtile em trows tcols (trc/(n/tcols)) (trc%(n/tcols))))
       (fun trc ->
         forall+ (_lid: natlt warp_size).
-          gpu_matrix_subtile gm trows tcols (trc/(cols/tcols)) (trc%(cols/tcols))
-            |-> Frac (f /. warp_size) (ematrix_subtile em trows tcols (trc/(cols/tcols)) (trc%(cols/tcols))))
+          gpu_matrix_subtile gm trows tcols (trc/(n/tcols)) (trc%(n/tcols))
+            |-> Frac (f /. warp_size) (ematrix_subtile em trows tcols (trc/(n/tcols)) (trc%(n/tcols))))
       fn trc { gpu_matrix_share_n _ warp_size };
-    forevery_unfactor' nthr (rows / trows * (cols / tcols)) 32 _;
+    forevery_unfactor' nthr (m / trows * (n / tcols)) 32 _;
     ();
   };
   forevery_map
     (fun (trc : natlt nblk) ->
-      (gpu_matrix_subtile gC (SZ.v bm) (SZ.v bn) (trc/(cols/bn)) (trc%(cols/bn)))
+      (gpu_matrix_subtile gC (SZ.v bm) (SZ.v bn) (trc/(n/bn)) (trc%(n/bn)))
         // Explicit fraction required, otherwise tactic to resolve it fails?!?!
         |-> Frac 1.0R
-      (ematrix_subtile eC bm bn (trc/(cols/bn)) (trc%(cols/bn))))
+      (ematrix_subtile eC bm bn (trc/(n/bn)) (trc%(n/bn))))
     _
     (fun trc ->
       create_warp_tiles_shared
         (block_tile gC (SZ.v bm) (SZ.v bn) trc)
-        // (gpu_matrix_subtile gC (SZ.v bm) (SZ.v bn) (trc/(cols/bn)) (trc%(cols/bn)))
+        // (gpu_matrix_subtile gC (SZ.v bm) (SZ.v bn) (trc/(n/bn)) (trc%(n/bn)))
         (wm*tm)
         (wn*tn)
         nthr);
@@ -314,7 +314,7 @@ fn setup
     (fun bid -> fun tid ->
       (warp_tile (block_tile gC (SZ.v bm) (SZ.v bn) bid) (wm*tm) (wn*tn) (tid/warp_size))
         |-> Frac (precip warp_size)
-      (ematrix_subtile (ematrix_subtile eC bm bn (bid/(cols/bn)) (bid%(cols/bn)))
+      (ematrix_subtile (ematrix_subtile eC bm bn (bid/(n/bn)) (bid%(n/bn)))
         (wm*tm) (wn*tn)
         (warp_tile_idx_rows (SZ.v bm) (SZ.v bn) (wm*tm) (wn*tn) (tid/warp_size))
         (warp_tile_idx_cols (SZ.v bm) (SZ.v bn) (wm*tm) (wn*tn) (tid/warp_size))));
@@ -330,7 +330,7 @@ fn setup
     gA |-> Frac (fA /. (nblk*nthr)) eA ** gB |-> Frac (fB /. (nblk*nthr)) eB **
     (warp_tile (block_tile gC (SZ.v bm) (SZ.v bn) bid) (wm*tm) (wn*tn) (tid/warp_size))
       |-> Frac (precip warp_size)
-    (ematrix_subtile (ematrix_subtile eC bm bn (bid/(cols/bn)) (bid%(cols/bn)))
+    (ematrix_subtile (ematrix_subtile eC bm bn (bid/(n/bn)) (bid%(n/bn)))
       (wm*tm) (wn*tn)
       (warp_tile_idx_rows (SZ.v bm) (SZ.v bn) (wm*tm) (wn*tn) (tid/warp_size))
       (warp_tile_idx_cols (SZ.v bm) (SZ.v bn) (wm*tm) (wn*tn) (tid/warp_size)))
@@ -349,34 +349,34 @@ fn block_setup
   (#et_ab #et_c : Type0)
   {| scalar et_ab, v : has_vec_cpy et_ab, scalar et_c |}
   {| real_like et_ab, real_like et_c |}
-  (#rows #shared #cols : szp)
-  (#lA : mlayout rows shared)
-  (#lB : mlayout shared cols)
-  (#lC : mlayout rows cols)
+  (#m #n #k : szp)
+  (#lA : mlayout m k)
+  (#lB : mlayout k n)
+  (#lC : mlayout m n)
   {| clayout lA, clayout lB, clayout lC |}
   (gA : gpu_matrix et_ab lA)
-  (eA : ematrix et_ab rows shared)
+  (eA : ematrix et_ab m k)
   (gB : gpu_matrix et_ab lB)
-  (eB : ematrix et_ab shared cols)
+  (eB : ematrix et_ab k n)
   (gC : gpu_matrix et_c lC)
-  (eC : ematrix et_c rows cols)
+  (eC : ematrix et_c m n)
   (bm bn bk
    tm tn tk
    wm wn : szp { constraints bm bn bk tm tn tk wm wn })
-  (#_ : squash (bm /?+ rows))
-  (#_ : squash (bk /?+ shared))
-  (#_ : squash (bn /?+ cols))
+  (#_ : squash (bm /?+ m))
+  (#_ : squash (bk /?+ k))
+  (#_ : squash (bn /?+ n))
   (#_ : squash (SZ.fits (bm * bk) /\ SZ.fits (bk * bn)))
-  (nblk : szp{SZ.v nblk == rows/bm * (cols/bn)})
+  (nblk : szp{SZ.v nblk == m/bm * (n/bn)})
   (nthr : szp{SZ.v nthr == bm/(wm*tm) * (bn/(wn*tn)) * warp_size /\ nthr <= 1024})
   (#_ : squash (chunk et_ab /?+ bn))
   (#_ : squash (chunk et_ab /?+ bk))
   (#_ : squash (chunk et_ab * nthr /?+ (bm * bk)))
   (#_ : squash (chunk et_ab * nthr /?+ (bk * bn)))
   (fA fB : perm)
-  (rA : ematrix real rows shared)
-  (rB : ematrix real shared cols)
-  (rC : ematrix real rows cols)
+  (rA : ematrix real m k)
+  (rB : ematrix real k n)
+  (rC : ematrix real m n)
   (sh : c_shmems (shmems_desc et_ab bm bn bk))
   (bid : natlt nblk)
   ()
@@ -405,31 +405,31 @@ fn block_teardown
   (#et_ab #et_c : Type0)
   {| scalar et_ab, has_vec_cpy et_ab, scalar et_c |}
   {| real_like et_ab, real_like et_c |}
-  (#rows #shared #cols : szp)
-  (#lA : mlayout rows shared)
-  (#lB : mlayout shared cols)
-  (#lC : mlayout rows cols)
+  (#m #n #k : szp)
+  (#lA : mlayout m k)
+  (#lB : mlayout k n)
+  (#lC : mlayout m n)
   (gA : gpu_matrix et_ab lA)
-  (eA : ematrix et_ab rows shared)
+  (eA : ematrix et_ab m k)
   (gB : gpu_matrix et_ab lB)
-  (eB : ematrix et_ab shared cols)
+  (eB : ematrix et_ab k n)
   (gC : gpu_matrix et_c lC)
-  (eC : ematrix et_c rows cols)
+  (eC : ematrix et_c m n)
   (bm bn bk
    tm tn tk
    wm wn : szp { constraints bm bn bk tm tn tk wm wn })
-  (#_ : squash (bm /?+ rows))
-  (#_ : squash (bk /?+ shared))
-  (#_ : squash (bn /?+ cols))
+  (#_ : squash (bm /?+ m))
+  (#_ : squash (bk /?+ k))
+  (#_ : squash (bn /?+ n))
   (#_ : squash (SZ.fits (bm * bk) /\ SZ.fits (bk * bn)))
-  (nblk : szp{SZ.v nblk == rows/bm * (cols/bn)})
+  (nblk : szp{SZ.v nblk == m/bm * (n/bn)})
   (nthr : szp{SZ.v nthr == bm/(wm*tm) * (bn/(wn*tn)) * warp_size})
   (fA fB : perm)
-  (rA : ematrix real rows shared)
-  (rB : ematrix real shared cols)
-  (rC : ematrix real rows cols)
-  (#_ : squash (wm * tm /?+ rows)) // obvious, but SMT is flaky
-  (#_ : squash (wn * tn /?+ cols)) // idem
+  (rA : ematrix real m k)
+  (rB : ematrix real k n)
+  (rC : ematrix real m n)
+  (#_ : squash (wm * tm /?+ m)) // obvious, but SMT is flaky
+  (#_ : squash (wn * tn /?+ n)) // idem
   (sh : c_shmems (shmems_desc et_ab bm bn bk))
   (bid : natlt nblk)
   ()
@@ -455,17 +455,17 @@ fn block_teardown
 ghost
 fn warp_tile_pts_to_eq
   (#et : Type0) {| scalar et |}
-  (#rows : nat)
-  (#cols : nat)
-  (#lC : mlayout rows cols)
+  (#m : nat)
+  (#n : nat)
+  (#lC : mlayout m n)
   (gC : gpu_matrix et lC)
-  (bm : pos{bm /?+ rows})
-  (bn : pos{bn /?+ cols})
+  (bm : pos{bm /?+ m})
+  (bn : pos{bn /?+ n})
   (tm : pos{tm /?+ bm})
   (tn : pos{tn /?+ bn})
   (wm : pos{wm * tm /?+ bm})
   (wn : pos{wn * tn /?+ bn})
-  (bid : natlt ((rows/bm) * (cols/bn)))
+  (bid : natlt ((m/bm) * (n/bn)))
   (wid : natlt (bm/(wm*tm) * (bn/(wn*tn))))
   (em1 em2 : ematrix et (wm * tm) (wn * tn))
   requires
@@ -488,17 +488,17 @@ fn warp_tile_pts_to_eq
 ghost
 fn warp_tile_pts_to_gatherwarp
   (#et : Type0) {| scalar et |}
-  (#rows : nat)
-  (#cols : nat)
-  (#lC : mlayout rows cols)
+  (#m : nat)
+  (#n : nat)
+  (#lC : mlayout m n)
   (gC : gpu_matrix et lC)
-  (bm : pos{bm /?+ rows})
-  (bn : pos{bn /?+ cols})
+  (bm : pos{bm /?+ m})
+  (bn : pos{bn /?+ n})
   (tm : pos{tm /?+ bm})
   (tn : pos{tn /?+ bn})
   (wm : pos{wm * tm /?+ bm})
   (wn : pos{wn * tn /?+ bn})
-  (bid : natlt ((rows/bm) * (cols/bn)))
+  (bid : natlt ((m/bm) * (n/bn)))
   (wid : natlt (bm/(wm*tm) * (bn/(wn*tn))))
   (em : ematrix et (wm * tm) (wn * tn))
   requires
@@ -529,25 +529,25 @@ fn rhs_is_constant_for_warps_approx
   (#et_ab #et_c : Type0)
   {| scalar et_c |}
   {| real_like et_c |}
-  (#rows #shared #cols : pos)
-  (#lC : mlayout rows cols)
+  (#m #n #k : pos)
+  (#lC : mlayout m n)
   (gC : gpu_matrix et_c lC)
-  (eA : ematrix et_ab rows shared)
-  (eB : ematrix et_ab shared cols)
-  (eC : ematrix et_c rows cols)
+  (eA : ematrix et_ab m k)
+  (eB : ematrix et_ab k n)
+  (eC : ematrix et_c m n)
   (bm bn bk
    tm tn tk
    wm wn : szp { constraints bm bn bk tm tn tk wm wn })
-  (#_ : squash (bm /?+ rows))
-  (#_ : squash (bn /?+ cols))
+  (#_ : squash (bm /?+ m))
+  (#_ : squash (bn /?+ n))
   (#_ : squash (SZ.fits (bm * bk) /\ SZ.fits (bk * bn)))
-  (nblk : pos{nblk == rows/bm * (cols/bn)})
+  (nblk : pos{nblk == m/bm * (n/bn)})
   (nthr : pos{nthr == bm/(wm*tm) * (bn/(wn*tn)) * warp_size})
-  (rA : ematrix real rows shared)
-  (rB : ematrix real shared cols)
-  (rC : ematrix real rows cols)
-  (#_ : squash (wm * tm /?+ rows)) // obvious, but SMT is flaky
-  (#_ : squash (wn * tn /?+ cols)) // idem
+  (rA : ematrix real m k)
+  (rB : ematrix real k n)
+  (rC : ematrix real m n)
+  (#_ : squash (wm * tm /?+ m)) // obvious, but SMT is flaky
+  (#_ : squash (wn * tn /?+ n)) // idem
   (bid : natlt nblk)
   (emf : natlt nthr -> ematrix et_c (wm*tm) (wn*tn))
   norewrite
@@ -555,14 +555,14 @@ fn rhs_is_constant_for_warps_approx
     forall+ (tid : natlt nthr).
       warp_tile_pts_to gC bm bn tm tn wm wn bid (tid / warp_size) (emf tid) **
       pure (emf tid %~
-        (MS.matmul (ematrix_subtile rA (wm*tm) shared (warp_tile_i #rows #cols bm bn bk tm tn tk wm wn nthr bid (tid / warp_size)) 0)
-                   (ematrix_subtile rB shared  (wn*tn) 0 (warp_tile_j #rows #cols bm bn bk tm tn tk wm wn nthr bid (tid / warp_size)))))
+        (MS.matmul (ematrix_subtile rA (wm*tm) k (warp_tile_i #m #n bm bn bk tm tn tk wm wn nthr bid (tid / warp_size)) 0)
+                   (ematrix_subtile rB k  (wn*tn) 0 (warp_tile_j #m #n bm bn bk tm tn tk wm wn nthr bid (tid / warp_size)))))
   ensures
     forall+ (wid : natlt (nthr / warp_size)).
       warp_tile_pts_to_full gC bm bn tm tn wm wn bid wid (emf (wid * warp_size)) **
       pure (emf (wid * warp_size) %~
-        (MS.matmul (ematrix_subtile rA (wm*tm) shared (warp_tile_i #rows #cols bm bn bk tm tn tk wm wn nthr bid wid) 0)
-                   (ematrix_subtile rB shared  (wn*tn) 0 (warp_tile_j #rows #cols bm bn bk tm tn tk wm wn nthr bid wid))))
+        (MS.matmul (ematrix_subtile rA (wm*tm) k (warp_tile_i #m #n bm bn bk tm tn tk wm wn nthr bid wid) 0)
+                   (ematrix_subtile rB k  (wn*tn) 0 (warp_tile_j #m #n bm bn bk tm tn tk wm wn nthr bid wid))))
 {
   forevery_factor nthr (nthr / warp_size) warp_size _;
   ghost
@@ -571,13 +571,13 @@ fn rhs_is_constant_for_warps_approx
       forall+ (i : natlt warp_size).
         warp_tile_pts_to gC bm bn tm tn wm wn bid ((wid * warp_size + i) / warp_size) (emf (wid * warp_size + i)) **
         pure (emf (wid * warp_size + i) %~
-          (MS.matmul (ematrix_subtile rA (wm*tm) shared (warp_tile_i #rows #cols bm bn bk tm tn tk wm wn nthr bid ((wid * warp_size + i) / warp_size)) 0)
-                     (ematrix_subtile rB shared  (wn*tn) 0 (warp_tile_j #rows #cols bm bn bk tm tn tk wm wn nthr bid ((wid * warp_size + i) / warp_size)))))
+          (MS.matmul (ematrix_subtile rA (wm*tm) k (warp_tile_i #m #n bm bn bk tm tn tk wm wn nthr bid ((wid * warp_size + i) / warp_size)) 0)
+                     (ematrix_subtile rB k  (wn*tn) 0 (warp_tile_j #m #n bm bn bk tm tn tk wm wn nthr bid ((wid * warp_size + i) / warp_size)))))
     ensures
       warp_tile_pts_to_full gC bm bn tm tn wm wn bid wid (emf (wid * warp_size)) **
       pure (emf (wid * warp_size) %~
-        (MS.matmul (ematrix_subtile rA (wm*tm) shared (warp_tile_i #rows #cols bm bn bk tm tn tk wm wn nthr bid wid) 0)
-                  (ematrix_subtile rB shared  (wn*tn) 0 (warp_tile_j #rows #cols bm bn bk tm tn tk wm wn nthr bid wid))))
+        (MS.matmul (ematrix_subtile rA (wm*tm) k (warp_tile_i #m #n bm bn bk tm tn tk wm wn nthr bid wid) 0)
+                  (ematrix_subtile rB k  (wn*tn) 0 (warp_tile_j #m #n bm bn bk tm tn tk wm wn nthr bid wid))))
   {
     forevery_natlt_pop_shift _ _;
 
@@ -589,15 +589,15 @@ fn rhs_is_constant_for_warps_approx
     // ghost
     // fn aux (tid : natlt
     // assert pure (em0 %~
-    //   (MS.matmul (ematrix_subtile rA (wm*tm) shared (warp_tile_i #rows #cols bm bn bk tm tn tk wm wn nthr bid ((wid * warp_size + i) / warp_size)) 0)
-    //              (ematrix_subtile rB shared  (wn*tn) 0 (warp_tile_j #rows #cols bm bn bk tm tn tk wm wn nthr bid ((wid * warp_size + i) / warp_size)))));
+    //   (MS.matmul (ematrix_subtile rA (wm*tm) k (warp_tile_i #m #n bm bn bk tm tn tk wm wn nthr bid ((wid * warp_size + i) / warp_size)) 0)
+    //              (ematrix_subtile rB k  (wn*tn) 0 (warp_tile_j #m #n bm bn bk tm tn tk wm wn nthr bid ((wid * warp_size + i) / warp_size)))));
     forevery_map_extra
       #(natlt (warp_size - 1))
       (warp_tile_pts_to gC bm bn tm tn wm wn bid wid em0)
       (fun i -> warp_tile_pts_to gC bm bn tm tn wm wn bid ((wid * warp_size + (i+1)) / warp_size) (emf (wid * warp_size + (i+1)))
         ** pure (emf (wid * warp_size + (i+1)) %~
-          (MS.matmul (ematrix_subtile rA (wm*tm) shared (warp_tile_i #rows #cols bm bn bk tm tn tk wm wn nthr bid ((wid * warp_size + (i+1)) / warp_size)) 0)
-                     (ematrix_subtile rB shared  (wn*tn) 0 (warp_tile_j #rows #cols bm bn bk tm tn tk wm wn nthr bid ((wid * warp_size + (i+1)) / warp_size))))))
+          (MS.matmul (ematrix_subtile rA (wm*tm) k (warp_tile_i #m #n bm bn bk tm tn tk wm wn nthr bid ((wid * warp_size + (i+1)) / warp_size)) 0)
+                     (ematrix_subtile rB k  (wn*tn) 0 (warp_tile_j #m #n bm bn bk tm tn tk wm wn nthr bid ((wid * warp_size + (i+1)) / warp_size))))))
       (fun i -> warp_tile_pts_to gC bm bn tm tn wm wn bid wid em0)
       // ^ NB: dropping the pure part above, it doesn't matter as we already have this fact about em0
       fn i {
@@ -626,46 +626,46 @@ let tiles_approx_lemma
   (#et_c : Type0)
   {| scalar et_c |}
   {| real_like et_c |}
-  (#rows #shared #cols : pos)
+  (#m #n #k : pos)
   (bm bn bk
    tm tn tk
    wm wn : szp { constraints bm bn bk tm tn tk wm wn })
-  (#_ : squash (bm /?+ rows))
-  (#_ : squash (bn /?+ cols))
+  (#_ : squash (bm /?+ m))
+  (#_ : squash (bn /?+ n))
   (#_ : squash (SZ.fits (bm * bk) /\ SZ.fits (bk * bn)))
-  (nblk : pos{nblk == rows/bm * (cols/bn)})
+  (nblk : pos{nblk == m/bm * (n/bn)})
   (nthr : pos{nthr == bm/(wm*tm) * (bn/(wn*tn)) * warp_size})
-  (rA : ematrix real rows shared)
-  (rB : ematrix real shared cols)
-  (#_ : squash (wm * tm /?+ rows)) // obvious, but SMT is flaky
-  (#_ : squash (wn * tn /?+ cols)) // idem
-  (eC' : ematrix et_c rows cols)
+  (rA : ematrix real m k)
+  (rB : ematrix real k n)
+  (#_ : squash (wm * tm /?+ m)) // obvious, but SMT is flaky
+  (#_ : squash (wn * tn /?+ n)) // idem
+  (eC' : ematrix et_c m n)
   (emf : natlt nblk -> natlt nthr -> ematrix et_c (wm*tm) (wn*tn))
   : Lemma (requires
             (eC' ==
               ematrix_from_tiles bm bn
                 (fun br bc ->
                   ematrix_from_tiles (wm*tm) (wn*tn)
-                    (fun tr tc -> emf (br * (cols/bn) + bc) ((tr * (bn/(wn*tn)) + tc) * warp_size))))
+                    (fun tr tc -> emf (br * (n/bn) + bc) ((tr * (bn/(wn*tn)) + tc) * warp_size))))
           /\ (forall (bid : natlt nblk) (wid : natlt (nthr / warp_size)).
                 emf bid (wid * warp_size) %~
-                  (MS.matmul (ematrix_subtile rA (wm*tm) shared (warp_tile_i #rows #cols bm bn bk tm tn tk wm wn nthr bid wid) 0)
-                            (ematrix_subtile rB shared  (wn*tn) 0 (warp_tile_j #rows #cols bm bn bk tm tn tk wm wn nthr bid wid)))))
+                  (MS.matmul (ematrix_subtile rA (wm*tm) k (warp_tile_i #m #n bm bn bk tm tn tk wm wn nthr bid wid) 0)
+                            (ematrix_subtile rB k  (wn*tn) 0 (warp_tile_j #m #n bm bn bk tm tn tk wm wn nthr bid wid)))))
           (ensures eC' %~ MS.matmul rA rB)
-= let aux (i : natlt rows) (j : natlt cols)
+= let aux (i : natlt m) (j : natlt n)
     : Lemma (macc eC' i j %~ macc (MS.matmul rA rB) i j)
   =
-    let bid : natlt nblk = bid_of_ij rows cols bm bn i j in
-    let wid : natlt (nthr / warp_size) = wid_of_ij rows cols bm bn tm tn wm wn i j in
+    let bid : natlt nblk = bid_of_ij m n bm bn i j in
+    let wid : natlt (nthr / warp_size) = wid_of_ij m n bm bn tm tn wm wn i j in
     let ii  : natlt (wm*tm) = (i % bm) % (wm*tm) in
     let jj  : natlt (wn*tn) = (j % bn) % (wn*tn) in
     calc (==) {
       macc eC' i j;
       == {}
-      macc (ematrix_from_tiles #_ #rows #cols bm bn
+      macc (ematrix_from_tiles #_ #m #n bm bn
               (fun br bc ->
                 ematrix_from_tiles (wm*tm) (wn*tn)
-                  (fun tr tc -> emf (br * (cols/bn) + bc) ((tr * (bn/(wn*tn)) + tc) * warp_size))))
+                  (fun tr tc -> emf (br * (n/bn) + bc) ((tr * (bn/(wn*tn)) + tc) * warp_size))))
         i j;
       == {}
       macc (ematrix_from_tiles #_ #bm #bn (wm*tm) (wn*tn)
@@ -677,19 +677,19 @@ let tiles_approx_lemma
     assert (macc eC' i j == macc (emf bid (wid * warp_size)) ii jj);
     assert (macc eC' i j %~
       macc
-        (MS.matmul (ematrix_subtile rA (wm*tm) shared (warp_tile_i #rows #cols bm bn bk tm tn tk wm wn nthr bid wid) 0)
-                   (ematrix_subtile rB shared  (wn*tn) 0 (warp_tile_j #rows #cols bm bn bk tm tn tk wm wn nthr bid wid)))
+        (MS.matmul (ematrix_subtile rA (wm*tm) k (warp_tile_i #m #n bm bn bk tm tn tk wm wn nthr bid wid) 0)
+                   (ematrix_subtile rB k  (wn*tn) 0 (warp_tile_j #m #n bm bn bk tm tn tk wm wn nthr bid wid)))
         ii jj);
 
-    MS.matmul_decompose_lemma rA rB (wm*tm) (wn*tn) (warp_tile_i #rows #cols bm bn bk tm tn tk wm wn nthr bid wid)
-                                                    (warp_tile_j #rows #cols bm bn bk tm tn tk wm wn nthr bid wid);
+    MS.matmul_decompose_lemma rA rB (wm*tm) (wn*tn) (warp_tile_i #m #n bm bn bk tm tn tk wm wn nthr bid wid)
+                                                    (warp_tile_j #m #n bm bn bk tm tn tk wm wn nthr bid wid);
     assert (macc eC' i j %~
       macc
         (ematrix_subtile
           (MS.matmul rA rB)
           (wm*tm) (wn*tn)
-          (warp_tile_i #rows #cols bm bn bk tm tn tk wm wn nthr bid wid)
-          (warp_tile_j #rows #cols bm bn bk tm tn tk wm wn nthr bid wid))
+          (warp_tile_i #m #n bm bn bk tm tn tk wm wn nthr bid wid)
+          (warp_tile_j #m #n bm bn bk tm tn tk wm wn nthr bid wid))
         ii jj);
 
     calc (==) {
@@ -697,16 +697,16 @@ let tiles_approx_lemma
         (ematrix_subtile
           (MS.matmul rA rB)
           (wm*tm) (wn*tn)
-          (warp_tile_i #rows #cols bm bn bk tm tn tk wm wn nthr bid wid)
-          (warp_tile_j #rows #cols bm bn bk tm tn tk wm wn nthr bid wid))
+          (warp_tile_i #m #n bm bn bk tm tn tk wm wn nthr bid wid)
+          (warp_tile_j #m #n bm bn bk tm tn tk wm wn nthr bid wid))
         ii jj;
       == {}
       macc
         (MS.matmul rA rB)
-        (warp_tile_i #rows #cols bm bn bk tm tn tk wm wn nthr bid wid * (wm*tm) + ii)
-        (warp_tile_j #rows #cols bm bn bk tm tn tk wm wn nthr bid wid * (wn*tn) + jj);
-      == { lem_i rows shared cols bm bn bk tm tn tk wm wn nthr i j;
-           lem_j rows shared cols bm bn bk tm tn tk wm wn nthr i j }
+        (warp_tile_i #m #n bm bn bk tm tn tk wm wn nthr bid wid * (wm*tm) + ii)
+        (warp_tile_j #m #n bm bn bk tm tn tk wm wn nthr bid wid * (wn*tn) + jj);
+      == { lem_i m n k bm bn bk tm tn tk wm wn nthr i j;
+           lem_j m n k bm bn bk tm tn tk wm wn nthr i j }
       macc (MS.matmul rA rB) i j;
     };
 
@@ -722,53 +722,53 @@ fn reconstruct_from_warp_approx
   (#et_ab #et_c : Type0)
   {| scalar et_c |}
   {| real_like et_c |}
-  (#rows #shared #cols : pos)
-  (#lC : mlayout rows cols)
+  (#m #n #k : pos)
+  (#lC : mlayout m n)
   (gC : gpu_matrix et_c lC)
-  (eA : ematrix et_ab rows shared)
-  (eB : ematrix et_ab shared cols)
-  (eC : ematrix et_c rows cols)
+  (eA : ematrix et_ab m k)
+  (eB : ematrix et_ab k n)
+  (eC : ematrix et_c m n)
   (bm bn bk
    tm tn tk
    wm wn : szp { constraints bm bn bk tm tn tk wm wn })
-  (#_ : squash (bm /?+ rows))
-  (#_ : squash (bn /?+ cols))
+  (#_ : squash (bm /?+ m))
+  (#_ : squash (bn /?+ n))
   (#_ : squash (SZ.fits (bm * bk) /\ SZ.fits (bk * bn)))
-  (nblk : pos{nblk == rows/bm * (cols/bn)})
+  (nblk : pos{nblk == m/bm * (n/bn)})
   (nthr : pos{nthr == bm/(wm*tm) * (bn/(wn*tn)) * warp_size})
-  (rA : ematrix real rows shared)
-  (rB : ematrix real shared cols)
-  (rC : ematrix real rows cols)
-  (#_ : squash (wm * tm /?+ rows)) // obvious, but SMT is flaky
-  (#_ : squash (wn * tn /?+ cols)) // idem
+  (rA : ematrix real m k)
+  (rB : ematrix real k n)
+  (rC : ematrix real m n)
+  (#_ : squash (wm * tm /?+ m)) // obvious, but SMT is flaky
+  (#_ : squash (wn * tn /?+ n)) // idem
   norewrite
   requires
     pure (SZ.fits (mlayout_size lC))
   requires
     forall+ (bid : natlt nblk) (tid : natlt nthr).
       warp_tile_approximates gC bm bn tm tn wm wn bid (tid / warp_size)
-        (MS.matmul (ematrix_subtile rA (wm*tm) shared (warp_tile_i #rows #cols bm bn bk tm tn tk wm wn nthr bid (tid / warp_size)) 0)
-                   (ematrix_subtile rB shared  (wn*tn) 0 (warp_tile_j #rows #cols bm bn bk tm tn tk wm wn nthr bid (tid / warp_size))))
+        (MS.matmul (ematrix_subtile rA (wm*tm) k (warp_tile_i #m #n bm bn bk tm tn tk wm wn nthr bid (tid / warp_size)) 0)
+                   (ematrix_subtile rB k  (wn*tn) 0 (warp_tile_j #m #n bm bn bk tm tn tk wm wn nthr bid (tid / warp_size))))
   ensures
-    exists* (eC' : ematrix et_c rows cols).
+    exists* (eC' : ematrix et_c m n).
       gC |-> eC' ** pure (eC' %~ MS.matmul rA rB)
 {
   (* Expose the existential. *)
   forevery_map_2 #(natlt nblk) #(natlt nthr)
     (fun bid tid ->
       warp_tile_approximates gC bm bn tm tn wm wn bid (tid / warp_size)
-        (MS.matmul (ematrix_subtile rA (wm*tm) shared (warp_tile_i #rows #cols bm bn bk tm tn tk wm wn nthr bid (tid / warp_size)) 0)
-                   (ematrix_subtile rB shared  (wn*tn) 0 (warp_tile_j #rows #cols bm bn bk tm tn tk wm wn nthr bid (tid / warp_size)))))
+        (MS.matmul (ematrix_subtile rA (wm*tm) k (warp_tile_i #m #n bm bn bk tm tn tk wm wn nthr bid (tid / warp_size)) 0)
+                   (ematrix_subtile rB k  (wn*tn) 0 (warp_tile_j #m #n bm bn bk tm tn tk wm wn nthr bid (tid / warp_size)))))
     (fun bid tid ->
       exists* (em : ematrix et_c (wm*tm) (wn*tn)).
         warp_tile_pts_to gC bm bn tm tn wm wn bid (tid / warp_size) em **
         pure (em %~
-          (MS.matmul (ematrix_subtile rA (wm*tm) shared (warp_tile_i #rows #cols bm bn bk tm tn tk wm wn nthr bid (tid / warp_size)) 0)
-                     (ematrix_subtile rB shared  (wn*tn) 0 (warp_tile_j #rows #cols bm bn bk tm tn tk wm wn nthr bid (tid / warp_size))))))
+          (MS.matmul (ematrix_subtile rA (wm*tm) k (warp_tile_i #m #n bm bn bk tm tn tk wm wn nthr bid (tid / warp_size)) 0)
+                     (ematrix_subtile rB k  (wn*tn) 0 (warp_tile_j #m #n bm bn bk tm tn tk wm wn nthr bid (tid / warp_size))))))
     fn bid tid {
       unfold warp_tile_approximates gC bm bn tm tn wm wn bid (tid / warp_size)
-        (MS.matmul (ematrix_subtile rA (wm*tm) shared (warp_tile_i #rows #cols bm bn bk tm tn tk wm wn nthr bid (tid / warp_size)) 0)
-                   (ematrix_subtile rB shared  (wn*tn) 0 (warp_tile_j #rows #cols bm bn bk tm tn tk wm wn nthr bid (tid / warp_size))));
+        (MS.matmul (ematrix_subtile rA (wm*tm) k (warp_tile_i #m #n bm bn bk tm tn tk wm wn nthr bid (tid / warp_size)) 0)
+                   (ematrix_subtile rB k  (wn*tn) 0 (warp_tile_j #m #n bm bn bk tm tn tk wm wn nthr bid (tid / warp_size))));
     };
 
   (* Choice. *)
@@ -776,21 +776,21 @@ fn reconstruct_from_warp_approx
     (fun (bid : natlt nblk) (tid : natlt nthr) (em : ematrix et_c (wm*tm) (wn*tn)) ->
         warp_tile_pts_to gC bm bn tm tn wm wn bid (tid / warp_size) em **
         pure (em %~
-          (MS.matmul (ematrix_subtile rA (wm*tm) shared (warp_tile_i #rows #cols bm bn bk tm tn tk wm wn nthr bid (tid / warp_size)) 0)
-                     (ematrix_subtile rB shared  (wn*tn) 0 (warp_tile_j #rows #cols bm bn bk tm tn tk wm wn nthr bid (tid / warp_size))))));
+          (MS.matmul (ematrix_subtile rA (wm*tm) k (warp_tile_i #m #n bm bn bk tm tn tk wm wn nthr bid (tid / warp_size)) 0)
+                     (ematrix_subtile rB k  (wn*tn) 0 (warp_tile_j #m #n bm bn bk tm tn tk wm wn nthr bid (tid / warp_size))))));
 
   (* Threads within a warp are uniform, factor and gather. *)
   forevery_map #(natlt nblk)
     (fun bid -> forall+ (tid : natlt nthr).
       warp_tile_pts_to gC bm bn tm tn wm wn bid (tid / warp_size) (emf bid tid) **
       pure (emf bid tid %~
-        (MS.matmul (ematrix_subtile rA (wm*tm) shared (warp_tile_i #rows #cols bm bn bk tm tn tk wm wn nthr bid (tid / warp_size)) 0)
-                   (ematrix_subtile rB shared  (wn*tn) 0 (warp_tile_j #rows #cols bm bn bk tm tn tk wm wn nthr bid (tid / warp_size))))))
+        (MS.matmul (ematrix_subtile rA (wm*tm) k (warp_tile_i #m #n bm bn bk tm tn tk wm wn nthr bid (tid / warp_size)) 0)
+                   (ematrix_subtile rB k  (wn*tn) 0 (warp_tile_j #m #n bm bn bk tm tn tk wm wn nthr bid (tid / warp_size))))))
     (fun bid -> forall+ (wid : natlt (nthr / warp_size)).
       warp_tile_pts_to_full gC bm bn tm tn wm wn bid wid (emf bid (wid * warp_size)) **
       pure (emf bid (wid * warp_size) %~
-        (MS.matmul (ematrix_subtile rA (wm*tm) shared (warp_tile_i #rows #cols bm bn bk tm tn tk wm wn nthr bid wid) 0)
-                   (ematrix_subtile rB shared  (wn*tn) 0 (warp_tile_j #rows #cols bm bn bk tm tn tk wm wn nthr bid wid)))))
+        (MS.matmul (ematrix_subtile rA (wm*tm) k (warp_tile_i #m #n bm bn bk tm tn tk wm wn nthr bid wid) 0)
+                   (ematrix_subtile rB k  (wn*tn) 0 (warp_tile_j #m #n bm bn bk tm tn tk wm wn nthr bid wid)))))
     fn bid {
       rhs_is_constant_for_warps_approx gC eA eB eC bm bn bk tm tn tk wm wn nblk nthr rA rB rC bid (emf bid);
     };
@@ -803,19 +803,19 @@ fn reconstruct_from_warp_approx
     (fun bid wid ->
       warp_tile_pts_to_full gC bm bn tm tn wm wn bid wid (emf bid (wid * warp_size)) **
       pure (emf bid (wid * warp_size) %~
-        (MS.matmul (ematrix_subtile rA (wm*tm) shared (warp_tile_i #rows #cols bm bn bk tm tn tk wm wn nthr bid wid) 0)
-                   (ematrix_subtile rB shared  (wn*tn) 0 (warp_tile_j #rows #cols bm bn bk tm tn tk wm wn nthr bid wid)))))
+        (MS.matmul (ematrix_subtile rA (wm*tm) k (warp_tile_i #m #n bm bn bk tm tn tk wm wn nthr bid wid) 0)
+                   (ematrix_subtile rB k  (wn*tn) 0 (warp_tile_j #m #n bm bn bk tm tn tk wm wn nthr bid wid)))))
     (fun bid wid ->
       emf bid (wid * warp_size) %~
-        (MS.matmul (ematrix_subtile rA (wm*tm) shared (warp_tile_i #rows #cols bm bn bk tm tn tk wm wn nthr bid wid) 0)
-                   (ematrix_subtile rB shared  (wn*tn) 0 (warp_tile_j #rows #cols bm bn bk tm tn tk wm wn nthr bid wid))))
+        (MS.matmul (ematrix_subtile rA (wm*tm) k (warp_tile_i #m #n bm bn bk tm tn tk wm wn nthr bid wid) 0)
+                   (ematrix_subtile rB k  (wn*tn) 0 (warp_tile_j #m #n bm bn bk tm tn tk wm wn nthr bid wid))))
     fn bid wid {
       ();
     };
   assert pure (forall (bid : natlt nblk) (wid : natlt (nthr / warp_size)).
     emf bid (wid * warp_size) %~
-      (MS.matmul (ematrix_subtile rA (wm*tm) shared (warp_tile_i #rows #cols bm bn bk tm tn tk wm wn nthr bid wid) 0)
-                 (ematrix_subtile rB shared  (wn*tn) 0 (warp_tile_j #rows #cols bm bn bk tm tn tk wm wn nthr bid wid))));
+      (MS.matmul (ematrix_subtile rA (wm*tm) k (warp_tile_i #m #n bm bn bk tm tn tk wm wn nthr bid wid) 0)
+                 (ematrix_subtile rB k  (wn*tn) 0 (warp_tile_j #m #n bm bn bk tm tn tk wm wn nthr bid wid))));
 
   (* Now drop the pures. *)
   forevery_map_2
@@ -823,8 +823,8 @@ fn reconstruct_from_warp_approx
     (fun bid wid ->
       warp_tile_pts_to_full gC bm bn tm tn wm wn bid wid (emf bid (wid * warp_size)) **
       pure (emf bid (wid * warp_size) %~
-        (MS.matmul (ematrix_subtile rA (wm*tm) shared (warp_tile_i #rows #cols bm bn bk tm tn tk wm wn nthr bid wid) 0)
-                   (ematrix_subtile rB shared  (wn*tn) 0 (warp_tile_j #rows #cols bm bn bk tm tn tk wm wn nthr bid wid)))))
+        (MS.matmul (ematrix_subtile rA (wm*tm) k (warp_tile_i #m #n bm bn bk tm tn tk wm wn nthr bid wid) 0)
+                   (ematrix_subtile rB k  (wn*tn) 0 (warp_tile_j #m #n bm bn bk tm tn tk wm wn nthr bid wid)))))
     (fun bid wid ->
       // warp_tile_pts_to_full gC bm bn tm tn wm wn bid wid (emf bid (wid * warp_size)))
       // gpu_matrix_pts_to
@@ -891,53 +891,53 @@ fn reconstruct_from_warp_approx
         (ematrix_from_tiles (wm*tm)
             (wn*tn)
             (fun tr tc -> emf bid ((tr * (bn/(wn*tn)) + tc) * 32))));
-  forevery_factor nblk (rows/bm) (cols/bn) _;
-  forevery_map_2 #(natlt (rows/bm)) #(natlt (cols/bn))
+  forevery_factor nblk (m/bm) (n/bn) _;
+  forevery_map_2 #(natlt (m/bm)) #(natlt (n/bn))
     (fun br bc ->
-      gpu_matrix_pts_to (block_tile gC (SZ.v bm) (SZ.v bn) (br * (cols/bn) + bc))
+      gpu_matrix_pts_to (block_tile gC (SZ.v bm) (SZ.v bn) (br * (n/bn) + bc))
         (ematrix_from_tiles (wm*tm) (wn*tn)
-            (fun tr tc -> emf (br * (cols/bn) + bc) ((tr * (bn/(wn*tn)) + tc) * 32))))
+            (fun tr tc -> emf (br * (n/bn) + bc) ((tr * (bn/(wn*tn)) + tc) * 32))))
     (fun br bc ->
       gpu_matrix_pts_to
         (gpu_matrix_subtile gC (SZ.v bm) (SZ.v bn) br bc)
         (ematrix_from_tiles (wm*tm) (wn*tn)
-            (fun tr tc -> emf (br * (cols/bn) + bc) ((tr * (bn/(wn*tn)) + tc) * 32))))
+            (fun tr tc -> emf (br * (n/bn) + bc) ((tr * (bn/(wn*tn)) + tc) * 32))))
     fn br bc {
       rewrite each
-        block_tile gC (SZ.v bm) (SZ.v bn) (br * (cols/bn) + bc)
+        block_tile gC (SZ.v bm) (SZ.v bn) (br * (n/bn) + bc)
       as
         gpu_matrix_subtile gC (SZ.v bm) (SZ.v bn)
-          (block_tile_idx_rows rows cols (SZ.v bm) (SZ.v bn) (br * (cols/bn) + bc))
-          (block_tile_idx_cols rows cols (SZ.v bm) (SZ.v bn) (br * (cols/bn) + bc));
+          (block_tile_idx_rows m n (SZ.v bm) (SZ.v bn) (br * (n/bn) + bc))
+          (block_tile_idx_cols m n (SZ.v bm) (SZ.v bn) (br * (n/bn) + bc));
       assert pure
-        (block_tile_idx_rows rows cols (SZ.v bm) (SZ.v bn) (br * (cols/bn) + bc)
+        (block_tile_idx_rows m n (SZ.v bm) (SZ.v bn) (br * (n/bn) + bc)
         ==
-        (br * (cols/bn) + bc) / (cols/bn)
+        (br * (n/bn) + bc) / (n/bn)
       );
-      assert pure ((br * (cols/bn) + bc) / (cols/bn) == br);
+      assert pure ((br * (n/bn) + bc) / (n/bn) == br);
       rewrite each
-        block_tile_idx_rows rows cols (SZ.v bm) (SZ.v bn) (br * (cols/bn) + bc)
+        block_tile_idx_rows m n (SZ.v bm) (SZ.v bn) (br * (n/bn) + bc)
       as
         br;
       assert pure (
-        block_tile_idx_cols rows cols (SZ.v bm) (SZ.v bn) (br * (cols/bn) + bc)
+        block_tile_idx_cols m n (SZ.v bm) (SZ.v bn) (br * (n/bn) + bc)
         ==
-        (br * (cols/bn) + bc) % (cols/bn)
+        (br * (n/bn) + bc) % (n/bn)
       );
-      assert pure ((br * (cols/bn) + bc) % (cols/bn) == bc);
+      assert pure ((br * (n/bn) + bc) % (n/bn) == bc);
       rewrite each
-        block_tile_idx_cols rows cols (SZ.v bm) (SZ.v bn) (br * (cols/bn) + bc)
+        block_tile_idx_cols m n (SZ.v bm) (SZ.v bn) (br * (n/bn) + bc)
       as
         bc;
 
       // These are needed to change the arguments to the implicit layout of gC...
-      rewrite each ((br * (cols/bn) + bc) / (cols/bn)) as br;
-      rewrite each ((br * (cols/bn) + bc) % (cols/bn)) as bc;
+      rewrite each ((br * (n/bn) + bc) / (n/bn)) as br;
+      rewrite each ((br * (n/bn) + bc) % (n/bn)) as bc;
 
       assert
         gpu_matrix_subtile gC (SZ.v bm) (SZ.v bn) br bc |->
           ematrix_from_tiles (wm*tm) (wn*tn)
-            (fun tr tc -> emf (br * (cols/bn) + bc) ((tr * (bn/(wn*tn)) + tc) * warp_size));
+            (fun tr tc -> emf (br * (n/bn) + bc) ((tr * (bn/(wn*tn)) + tc) * warp_size));
 
       ();
     };
@@ -945,7 +945,7 @@ fn reconstruct_from_warp_approx
   gpu_matrix_untile' gC bm bn
     (fun br bc ->
       ematrix_from_tiles (wm*tm) (wn*tn)
-        (fun tr tc -> emf (br * (cols/bn) + bc) ((tr * (bn/(wn*tn)) + tc) * warp_size)));
+        (fun tr tc -> emf (br * (n/bn) + bc) ((tr * (bn/(wn*tn)) + tc) * warp_size)));
 
   (* We now have full permission of gC. We now need to prove the
      functional post. *)
@@ -963,33 +963,33 @@ fn teardown
   (#et_ab #et_c : Type0)
   {| scalar et_ab, has_vec_cpy et_ab, scalar et_c |}
   {| real_like et_ab, real_like et_c |}
-  (#rows #shared #cols : szp)
-  (#lA : mlayout rows shared)
-  (#lB : mlayout shared cols)
-  (#lC : mlayout rows cols)
+  (#m #n #k : szp)
+  (#lA : mlayout m k)
+  (#lB : mlayout k n)
+  (#lC : mlayout m n)
   (gA : gpu_matrix et_ab lA)
-  (eA : ematrix et_ab rows shared)
+  (eA : ematrix et_ab m k)
   (gB : gpu_matrix et_ab lB)
-  (eB : ematrix et_ab shared cols)
+  (eB : ematrix et_ab k n)
   (gC : gpu_matrix et_c lC)
-  (eC : ematrix et_c rows cols)
+  (eC : ematrix et_c m n)
   (bm bn bk
    tm tn tk
    wm wn : szp { constraints bm bn bk tm tn tk wm wn })
-  (#_ : squash (bm /?+ rows))
-  (#_ : squash (bk /?+ shared))
-  (#_ : squash (bn /?+ cols))
+  (#_ : squash (bm /?+ m))
+  (#_ : squash (bk /?+ k))
+  (#_ : squash (bn /?+ n))
   (#_ : squash (SZ.fits (bm * bk) /\ SZ.fits (bk * bn)))
-  (nblk : szp{SZ.v nblk == rows/bm * (cols/bn)})
+  (nblk : szp{SZ.v nblk == m/bm * (n/bn)})
   (nthr : szp{SZ.v nthr == bm/(wm*tm) * (bn/(wn*tn)) * warp_size})
   (#_ : squash (chunk et_ab * nthr /?+ (bm * bk)))
   (#_ : squash (chunk et_ab * nthr /?+ (bk * bn)))
   (fA fB : perm)
-  (rA : ematrix real rows shared)
-  (rB : ematrix real shared cols)
-  (rC : ematrix real rows cols)
-  (#_ : squash (wm * tm /?+ rows)) // obvious, but SMT is flaky
-  (#_ : squash (wn * tn /?+ cols)) // idem
+  (rA : ematrix real m k)
+  (rB : ematrix real k n)
+  (rC : ematrix real m n)
+  (#_ : squash (wm * tm /?+ m)) // obvious, but SMT is flaky
+  (#_ : squash (wn * tn /?+ n)) // idem
   ()
   norewrite
   requires
@@ -1000,35 +1000,35 @@ fn teardown
   ensures
     gA |-> Frac fA eA **
     gB |-> Frac fB eB **
-    (exists* (eC' : ematrix et_c rows cols).
+    (exists* (eC' : ematrix et_c m n).
       gC |-> eC' ** pure (eC' %~ MS.matmul rA rB))
 {
-  forevery_unfactor' (rows/bm * (cols/bn) * nthr) nblk nthr _;
+  forevery_unfactor' (m/bm * (n/bn) * nthr) nblk nthr _;
   forevery_unzip _ _;
   forevery_unzip _ _;
 
-  gpu_matrix_gather_n gA (rows/bm * (cols/bn) * nthr);
-  gpu_matrix_gather_n gB (rows/bm * (cols/bn) * nthr);
+  gpu_matrix_gather_n gA (m/bm * (n/bn) * nthr);
+  gpu_matrix_gather_n gB (m/bm * (n/bn) * nthr);
 
   (* Done with gA and gB. The tricky bit is getting back gC and
   proving it approximates the matmul. *)
 
-  assert forall+ (x : natlt (rows / bm * (cols / bn) * nthr)).
+  assert forall+ (x : natlt (m / bm * (n / bn) * nthr)).
     warp_tile_approximates gC bm bn tm tn wm wn (x / nthr) (x % nthr / warp_size)
-      (MS.matmul (ematrix_subtile rA (wm*tm) shared (warp_tile_i bm bn bk tm tn tk wm wn nthr (x / nthr) (x % nthr / warp_size)) 0)
-                 (ematrix_subtile rB shared  (wn*tn) 0 (warp_tile_j bm bn bk tm tn tk wm wn nthr (x / nthr) (x % nthr / warp_size))));
+      (MS.matmul (ematrix_subtile rA (wm*tm) k (warp_tile_i bm bn bk tm tn tk wm wn nthr (x / nthr) (x % nthr / warp_size)) 0)
+                 (ematrix_subtile rB k  (wn*tn) 0 (warp_tile_j bm bn bk tm tn tk wm wn nthr (x / nthr) (x % nthr / warp_size))));
 
   forevery_factor'
-    (rows/bm * (cols/bn) * nthr)
-    (rows/bm * (cols/bn))
+    (m/bm * (n/bn) * nthr)
+    (m/bm * (n/bn))
     nthr
-    (fun (bid : natlt (rows/bm * (cols/bn))) (tid : natlt nthr) ->
+    (fun (bid : natlt (m/bm * (n/bn))) (tid : natlt nthr) ->
       warp_tile_approximates gC bm bn tm tn wm wn bid (tid / warp_size)
-        (MS.matmul (ematrix_subtile rA (wm*tm) shared (warp_tile_i bm bn bk tm tn tk wm wn nthr bid (tid / warp_size)) 0)
-                  (ematrix_subtile rB shared  (wn*tn) 0 (warp_tile_j bm bn bk tm tn tk wm wn nthr bid (tid / warp_size)))));
+        (MS.matmul (ematrix_subtile rA (wm*tm) k (warp_tile_i bm bn bk tm tn tk wm wn nthr bid (tid / warp_size)) 0)
+                  (ematrix_subtile rB k  (wn*tn) 0 (warp_tile_j bm bn bk tm tn tk wm wn nthr bid (tid / warp_size)))));
 
   reconstruct_from_warp_approx
-    gC eA eB eC bm bn bk tm tn tk wm wn (rows/bm * (cols/bn)) nthr rA rB rC;
+    gC eA eB eC bm bn bk tm tn tk wm wn (m/bm * (n/bn)) nthr rA rB rC;
 
   ();
 }
