src/klas/Klas.GEMM.BlockTiling2D.Inst.fst
@@ -27,15 +27,15 @@ fn spec
   (#_ : squash (chunk et * (bm/tm * (bn/tn)) /?+ (bm * bk)))
   (#_ : squash (chunk et * (bm/tm * (bn/tn)) /?+ (bk * bn)))
   (alpha beta : et)
-  (#rows #shared #cols : szp)
-  (gA : array2 et (rm rows shared) { is_global gA })
+  (#m #n #k : szp)
+  (gA : array2 et (rm m k) { is_global gA })
   (#fA : perm)
-  (gB : array2 et (rm shared cols) { is_global gB })
+  (gB : array2 et (rm k n) { is_global gB })
   (#fB : perm)
-  (gC : array2 et (rm rows cols) { is_global gC })
-  (#eA : ematrix et rows shared)
-  (#eB : ematrix et shared cols)
-  (#eC : ematrix et rows cols)
+  (gC : array2 et (rm m n) { is_global gC })
+  (#eA : ematrix et m k)
+  (#eB : ematrix et k n)
+  (#eC : ematrix et m n)
   norewrite
   preserves
     cpu **
@@ -44,7 +44,7 @@ fn spec
   requires
     pure (aligned 16 (core gA)) **
     pure (aligned 16 (core gB)) **
-    pure (rows * cols <= max_blocks) **
+    pure (m * n <= max_blocks) **
     on gpu_loc (gC |-> eC)
   ensures
     on gpu_loc (gC |-> MS.gemm alpha beta eC eA eB)
@@ -63,32 +63,32 @@ fn spec
   dassert (tm >^ 0sz);
   dassert (bm %^ tm = 0sz);
   dassert (bn %^ tn = 0sz);
-  dguard (rows   %^ bm = 0sz);
-  dguard (shared %^ bk = 0sz);
-  dguard (cols   %^ bn = 0sz);
-  let mrows   = rows   /^ bm;
-  let mshared = shared /^ bk;
-  let mcols   = cols   /^ bn;
+  dguard (m   %^ bm = 0sz);
+  dguard (k %^ bk = 0sz);
+  dguard (n   %^ bn = 0sz);
+  let mrows   = m /^ bm;
+  let mshared = k /^ bk;
+  let mcols   = n /^ bn;
 
-  lemma_divides_trans (chunk et) bk shared;
-  assert pure (chunk et /?+ shared);
-  lemma_aligned_strided_row_major_l2_row_major #(SZ.v rows) #(SZ.v shared) (chunk et);
+  lemma_divides_trans (chunk et) bk k;
+  assert pure (chunk et /?+ k);
+  lemma_aligned_strided_row_major_l2_row_major #(SZ.v m) #(SZ.v k) (chunk et);
 
-  lemma_divides_trans (chunk et) bn cols;
-  assert pure (chunk et /?+ cols);
-  lemma_aligned_strided_row_major_l2_row_major #(SZ.v shared) #(SZ.v cols) (chunk et);
+  lemma_divides_trans (chunk et) bn n;
+  assert pure (chunk et /?+ n);
+  lemma_aligned_strided_row_major_l2_row_major #(SZ.v k) #(SZ.v n) (chunk et);
 
   assert pure (SZ.fits (bm * bk));
   assert pure (SZ.fits (bk * bn));
 
-  assert pure (rows / bm <= rows);
-  assert pure (cols / bn <= cols);
-  assert pure ((rows / bm) * (cols / bn) <= rows * cols);
-  assert pure ((rows / bm) * (cols / bn) <= max_blocks);
+  assert pure (m / bm <= m);
+  assert pure (n / bn <= n);
+  assert pure ((m / bm) * (n / bn) <= m * n);
+  assert pure ((m / bm) * (n / bn) <= max_blocks);
 
   K.mmcomb_gpu_exact
     (fun o n -> mul beta o `add` mul alpha n)
-    #rows #shared #cols
+    #m #n #k
     gA #eA gB #eB gC #eC
     bm bn bk
     tm tn
