src/klas/Klas.GEMM.BlockTiling2D.Inst.fsti
@@ -17,8 +17,6 @@ let sz_fits (x:int) = 0 <= x /\ x < 4294967296
 inline_for_extraction noextract
 fn spec
   (bm bn bk : szp)
-  // These are fixed, by this function, to column-major and row-major
-  // respectively, which is the more efficient thing to do.
   (tm : szp{tm /? bm})
   (tn : szp{tn /? bn /\ (bm/tm * bn/tn <= max_threads)})
   (#_ : squash (sz_fits (bm*bk + (bm/tm * (bn/tn)))))
@@ -29,15 +27,15 @@ fn spec
   (#_ : squash (chunk et * (bm/tm * (bn/tn)) /?+ (bm * bk)))
   (#_ : squash (chunk et * (bm/tm * (bn/tn)) /?+ (bk * bn)))
   (alpha beta : et)
-  (#rows #shared #cols : szp)
-  (gA : array2 et (rm rows shared) { is_global gA })
+  (#m #n #k : szp)
+  (gA : array2 et (rm m k) { is_global gA })
   (#fA : perm)
-  (gB : array2 et (rm shared cols) { is_global gB })
+  (gB : array2 et (rm k n) { is_global gB })
   (#fB : perm)
-  (gC : array2 et (rm rows cols) { is_global gC })
-  (#eA : ematrix et rows shared)
-  (#eB : ematrix et shared cols)
-  (#eC : ematrix et rows cols)
+  (gC : array2 et (rm m n) { is_global gC })
+  (#eA : ematrix et m k)
+  (#eB : ematrix et k n)
+  (#eC : ematrix et m n)
   norewrite
   preserves
     cpu **
@@ -46,7 +44,7 @@ fn spec
   requires
     pure (aligned 16 (core gA)) **
     pure (aligned 16 (core gB)) **
-    pure (rows * cols <= max_blocks) **
+    pure (m * n <= max_blocks) **
     on gpu_loc (gC |-> eC)
   ensures
     on gpu_loc (gC |-> MS.gemm alpha beta eC eA eB)
