src/lib/kernel/gemm/Kuiper.Kernel.GEMM.TensorCore.fsti
@@ -16,21 +16,21 @@ inline_for_extraction noextract
 val mk_kernel
   (#et_ab #et_c : Type0)
   {| scalar et_ab, has_vec_cpy et_ab, scalar et_c |}
-  (#rows #shared #cols : szp)
-  (#lA : mlayout rows shared) {| clayout lA, str_A : strided_row_major lA |}
+  (#m #n #k : szp)
+  (#lA : mlayout m k) {| clayout lA, str_A : strided_row_major lA |}
   (gA : gpu_matrix et_ab lA { is_global gA })
-  (#eA : ematrix et_ab rows shared)
-  (#lB : mlayout shared cols) {| clayout lB, str_B : strided_row_major lB |}
+  (#eA : ematrix et_ab m k)
+  (#lB : mlayout k n) {| clayout lB, str_B : strided_row_major lB |}
   (#_ : squash (aligned_strided_row_major (chunk et_ab) str_A))
   (#_ : squash (aligned_strided_row_major (chunk et_ab) str_B))
   (gB : gpu_matrix et_ab lB { is_global gB })
-  (#eB : ematrix et_ab shared cols)
-  (gC : gpu_matrix et_c (row_major rows cols) { is_global gC })
-  (#_ : squash (SZ.fits (rows * cols)))
-  (#eC : ematrix et_c rows cols)
-  (bm : szp{bm /?+ rows})
-  (bn : szp{bn /?+ cols})
-  (bk : szp{bk /?+ shared})
+  (#eB : ematrix et_ab k n)
+  (gC : gpu_matrix et_c (row_major m n) { is_global gC })
+  (#_ : squash (SZ.fits (m * n)))
+  (#eC : ematrix et_c m n)
+  (bm : szp{bm /?+ m})
+  (bn : szp{bn /?+ n})
+  (bk : szp{bk /?+ k})
   (#_ : squash (chunk et_ab /?+ bn))
   (#_ : squash (chunk et_ab /?+ bk))
   (#_: squash (SZ.fits (bm * bk) /\ SZ.fits (bk * bn)))
@@ -38,7 +38,7 @@ val mk_kernel
   (tn : szp{tn /?+ bn})
   (tk : szp{tk /?+ bk})
   (#fA #fB : perm)
-  (nblk : szp{SZ.v nblk == rows/bm * (cols/bn)})
+  (nblk : szp{SZ.v nblk == m/bm * (n/bn)})
   // WARNING the previous version was wrong, it was assuming that each
   //  thread computes tm*tk results similar to 2D-Blocktiling.
   // There is nothing that catches this.
