src/lib/kernel/gemm/Kuiper.Kernel.GEMM.Tiled.Common.Vec.fsti
@@ -31,26 +31,26 @@ let shmems_desc
 inline_for_extraction noextract
 fn copy_tiles_out_of_matrices_vec
   (#et : Type0) {| scalar et, has_vec_cpy et |}
-  (#rows #shared #cols : erased nat)
-  (bm : szp{bm /? rows})
-  (bn : szp{bn /? cols})
-  (bk : szp{bk /? shared})
+  (#m #n #k : erased nat)
+  (bm : szp{bm /? m})
+  (bn : szp{bn /? n})
+  (bk : szp{bk /? k})
   (#_ : squash (chunk et /? bk)) // extra req
   (#_ : squash (chunk et /? bn)) // extra req
   (#slA : mlayout bm bk) {| clayout slA |}
   (#slB : mlayout bk bn) {| clayout slB |}
   (sA : gpu_matrix et slA)
   (sB : gpu_matrix et slB)
-  (#lA : mlayout rows shared) {| clayout lA, str_A : strided_row_major lA |}
-  (#lB : mlayout shared cols) {| clayout lB, str_B : strided_row_major lB |}
+  (#lA : mlayout m k) {| clayout lA, str_A : strided_row_major lA |}
+  (#lB : mlayout k n) {| clayout lB, str_B : strided_row_major lB |}
   (gA : gpu_matrix et lA)
-  (#eA : ematrix et rows shared)
+  (#eA : ematrix et m k)
   (gB : gpu_matrix et lB)
   (#fA #fB : perm)
-  (#eB : ematrix et shared cols)
-  (tile_row : szlt (rows/bm))
-  (tile_shared : szlt (shared/bk))
-  (tile_col : szlt (cols/bn))
+  (#eB : ematrix et k n)
+  (tile_row : szlt (m/bm))
+  (tile_shared : szlt (k/bk))
+  (tile_col : szlt (n/bn))
   (nthr : szp)
   (#_ : squash (chunk et * nthr /?+ (bm * bk))) // extra req
   (#_ : squash (chunk et * nthr /?+ (bk * bn))) // extra req
@@ -76,22 +76,22 @@ fn copy_tiles_out_of_matrices_vec
 
 unfold
 let block_tile_idx_rows
-  (rows cols : erased nat)
-  (bm : erased nat {bm > 0 /\ bm /? rows})
-  (bn : erased nat {bn > 0 /\ bn /? cols})
-  (bid : enatlt (rows/bm * (cols/bn)))
-  : enatlt (rows/bm)
+  (m n : erased nat)
+  (bm : erased nat {bm > 0 /\ bm /? m})
+  (bn : erased nat {bn > 0 /\ bn /? n})
+  (bid : enatlt (m/bm * (n/bn)))
+  : enatlt (m/bm)
   =
-    bid / (cols/bn)
+    bid / (n/bn)
 
 unfold
 let block_tile_idx_cols
-  (rows cols : erased nat)
-  (bm : erased nat {bm > 0 /\ bm /? rows})
-  (bn : erased nat {bn > 0 /\ bn /? cols})
-  (bid : enatlt (rows/bm * (cols/bn)))
-  : enatlt (cols/bn)
-  = bid % (cols/bn)
+  (m n : erased nat)
+  (bm : erased nat {bm > 0 /\ bm /? m})
+  (bn : erased nat {bn > 0 /\ bn /? n})
+  (bid : enatlt (m/bm * (n/bn)))
+  : enatlt (n/bn)
+  = bid % (n/bn)
 
 unfold
 let thread_tile_idx_rows
@@ -114,20 +114,20 @@ let thread_tile_idx_cols
 inline_for_extraction noextract
 let block_tile
   (#et : Type0)
-  (#rows #cols : erased nat)
-  (#lC : mlayout rows cols)
+  (#m #n : erased nat)
+  (#lC : mlayout m n)
   (gC : gpu_matrix et lC)
-  (bm : erased nat{bm > 0 /\ bm /? rows})
-  (bn : erased nat{bn > 0 /\ bn /? cols})
-  (bid : enatlt (rows/bm * (cols/bn)))
+  (bm : erased nat{bm > 0 /\ bm /? m})
+  (bn : erased nat{bn > 0 /\ bn /? n})
+  (bid : enatlt (m/bm * (n/bn)))
   : Tot (gpu_matrix et
           (subtile_layout lC bm bn
-            (block_tile_idx_rows rows cols bm bn bid)
-            (block_tile_idx_cols rows cols bm bn bid)))
+            (block_tile_idx_rows m n bm bn bid)
+            (block_tile_idx_cols m n bm bn bid)))
   =
     gpu_matrix_subtile gC bm bn
-      (block_tile_idx_rows rows cols bm bn bid)
-      (block_tile_idx_cols rows cols bm bn bid)
+      (block_tile_idx_rows m n bm bn bid)
+      (block_tile_idx_cols m n bm bn bid)
 
 inline_for_extraction noextract
 let thread_tile
